lpht: implement update-and-delete-older update logic for zombie case and add proof infrastructure for incorporating the new logic

pulse/share/steel/examples/pulse/dice/lib/LinearScanHashTable.fst
@@ -176,29 +176,36 @@ let used_upd_lookup_walk #s #sz (spec1 spec2 : spec_t s) (repr1 repr2 : repr_t s
   in
   aux 0
 
-let upd_and_delete_older #s #sz (spec : erased (spec_t s)) (repr : repr_t s sz{pht_models s sz spec repr}) idx k v
-: r':repr_t s sz{pht_models s sz (spec ++ (k,v)) r'}
-// the logic is tricky, we need to insert here, and keep going to find 
-// an older occurrence of the key and delete it (mark it as a zombie)
-// e.g., assume A and C hash to the same bucket and the table is:
-//
-//  A
-//  zombie
-//  C
-//
-// And we try to insert C: we cannot just put it in the zombie,
-// we need to delete the one below too.
-// admit ()
-  = admit()
+let del_ #s #sz (repr : repr_t s sz) idx : repr_t s sz =
+  Seq.upd repr idx Zombie
 
-let zombie_upd_lookup_walk #s #sz (spec1 spec2 : spec_t s) (repr1 repr2 : repr_t s sz) idx k v (k':_{k =!= k'})
+let upd_and_delete_older #s #sz (spec : erased (spec_t s)) (repr : repr_t s sz) cidx off0 k v
+  : r':repr_t s sz
+  = let repr' = upd_ repr ((cidx + off0) % sz) k v in
+    let rec aux (off:nat{off <= sz}) 
+      : Tot (repr_t s sz)
+            (decreases sz - off) 
+      = if off = sz then repr
+        else begin
+          let idx' = (cidx + off) % sz in
+          match repr @@ idx' with
+          | Clean -> repr
+          | Used k' v' ->
+            if k = k' then del_ repr idx'
+            else aux (off+1)
+          | Zombie ->
+            aux (off+1)
+        end
+    in
+    aux off0
+
+let zombie_upd_lookup_walk #s #sz (spec1 spec2 : spec_t s) (repr1 repr2 : repr_t s sz) cidx off k v (k':_{k =!= k'})
   : Lemma (requires
-      (forall i. i < sz /\ i <> idx ==> repr1 @@ i == repr2 @@ i)
-      /\ pht_models s sz spec1 repr1
-      /\ repr1 @@ idx == Zombie
-      // /\ repr2 @@ idx == Used k v // reundandant, given precondition below
-      /\ repr2 == upd_and_delete_older spec1 repr1 idx k v
-      /\ spec2 == spec1 ++ (k,v))
+      forall i. i < sz /\ i <> (cidx + off) % sz ==> repr1 @@ i == repr2 @@ i /\ // not true: might delete an old (k,v') at some i
+      pht_models s sz spec1 repr1 /\
+      repr1 @@ (cidx + off) % sz == Zombie /\
+      repr2 == upd_and_delete_older spec1 repr1 cidx off k v /\
+      spec2 == spec1 ++ (k,v))
       (ensures lookup_repr repr1 k' == lookup_repr repr2 k')
 = let idx' = canonical_index k' sz in
   let rec aux (off:nat{off <= sz}) : Lemma
@@ -208,19 +215,16 @@ let zombie_upd_lookup_walk #s #sz (spec1 spec2 : spec_t s) (repr1 repr2 : repr_t
         (decreases sz - off) 
   =
     if off = sz then ()
-    else if (idx' + off) % sz = idx then
-      begin
-        admit();
-        aux (off+1)
-      end
+    else if (idx' + off) % sz = (cidx + off) % sz then
+      admit()
     else begin
-      match repr1 @@ ((idx' + off) % sz) with
+      match repr1 @@ (idx' + off) % sz with
       | Clean -> ()
       | Used k'' v'' ->
         if k' = k'' then ()
         else aux (off+1)
       | Zombie ->
-        aux (off+1)
+        admit()
     end
   in
   aux 0
@@ -315,32 +319,32 @@ let used_upd #s #sz spec (repr : repr_t s sz{pht_models s sz spec repr}) idx k (
     Classical.forall_intro (Classical.move_requires aux2);
     Classical.forall_intro_3 (Classical.move_requires_3 aux3)
 
-let zombie_upd #s #sz spec (repr : repr_t s sz{pht_models s sz spec repr}) idx k v
+let zombie_upd #s #sz spec (repr : repr_t s sz{pht_models s sz spec repr}) cidx off k v
   : Lemma
-       (requires repr @@ idx == Zombie
-              /\ all_used_not_by repr (canonical_index k sz) idx k)
-       (ensures pht_models s sz (spec ++ (k,v)) (upd_and_delete_older spec repr idx k v))
+       (requires repr @@ (cidx + off) % sz == Zombie
+              /\ all_used_not_by repr (canonical_index k sz) ((cidx + off) % sz) k)
+       (ensures pht_models s sz (spec ++ (k,v)) (upd_and_delete_older spec repr cidx off k v))
   = let spec' = spec ++ (k,v) in
-    let repr' = upd_and_delete_older spec repr idx k v in
+    let repr' = upd_and_delete_older spec repr cidx off k v in
     let aux1 (k':s.keyt) : Lemma (requires (Some? (lookup_spec spec' k')))
                                  (ensures (lookup_repr repr' k' == lookup_spec spec' k'))
     = if k' = k then
+        // FIXME: need a lemma similar to lem_walk_from_canonical_all_used but specific to 
+        // the update given by upd_and_delete_older instead of upd_
         admit()
       else
-        begin
-          assume (forall i. i < sz /\ i <> idx ==> repr @@ i == repr' @@ i);
-          zombie_upd_lookup_walk spec spec' repr repr' idx k v k'
-        end
+        admit(); // FIXME: precondition of following lemma is false 
+        zombie_upd_lookup_walk spec spec' repr repr' cidx off k v k'
     in
     let aux2 (k':s.keyt) : Lemma (requires (Some? (lookup_repr repr' k')))
                                  (ensures (lookup_repr repr' k' == lookup_spec spec' k'))
     = if k' = k then
+        // FIXME: need a lemma similar to lem_walk_from_canonical_all_used but specific to 
+        // the update given by upd_and_delete_older instead of upd_
         admit()
       else
-        begin
-          assume (forall i. i < sz /\ i <> idx ==> repr @@ i == repr' @@ i);
-          zombie_upd_lookup_walk spec spec' repr repr' idx k v k'
-        end
+        admit(); // FIXME: precondition of following lemma is false
+        zombie_upd_lookup_walk spec spec' repr repr' cidx off k v k'
     in
     let aux3 (i':nat{i' < Seq.Base.length repr'}) (k':s.keyt) (v':s.valt) : Lemma (requires (repr' @@ i' == Used k' v'))
                                                                                   (ensures (lookup_repr_index repr' k' == Some (v', i')))
@@ -357,8 +361,7 @@ let insert_repr #s #sz (#spec : erased (spec_t s)) (repr : repr_t s sz{pht_model
                                      (_ : squash (walk repr cidx k off == lookup_repr repr k))
     : Tot (repr':repr_t s sz{pht_models s sz (spec ++ (k,v)) repr'})
           (decreases sz - off)
-    =
-      if off = sz then admit() // FIXME: table full, need side condition
+    = if off = sz then admit () // FIXME: table full, need side condition
       else
       let idx = (cidx+off) % sz in
       match repr @@ idx with
@@ -375,8 +378,8 @@ let insert_repr #s #sz (#spec : erased (spec_t s)) (repr : repr_t s sz{pht_model
         clean_upd spec repr idx k v;
         upd_ repr idx k v
       | Zombie ->
-        zombie_upd spec repr idx k v;
-        upd_and_delete_older spec repr idx k v
+        zombie_upd spec repr cidx off k v;
+        upd_and_delete_older spec repr cidx off k v
   in
   let res = walk_ 0 () () in
   res
